LeanTrominoes.lean
@@ -45,6 +45,7 @@ import LeanTrominoes.PartrecBinaryLengthSpace
 import LeanTrominoes.PartrecCodeSpace
 import LeanTrominoes.PartrecFlatIteration
 import LeanTrominoes.PartrecFlatIterationSpace
+import LeanTrominoes.PartrecFuel
 import LeanTrominoes.PartrecListCode
 import LeanTrominoes.PartrecListCodeSpace
 import LeanTrominoes.PartrecPolySpace
